test.v
@@ -1,0 +1,46 @@
+Require Import ssreflect.
+Generalizable All Variables.
+Typeclasses eauto := 1.
+
+Record Test := { c: Type }.
+
+Canonical build : Test :=
+  {|
+    c := Type
+  |}
+.
+
+Print Canonical Projections.
+
+Check (forall Q: c _, option Q).
+
+(* On the other hand, the following fails!
+Check (forall Q: c _, Q -> Q). 
+But that works:
+Check (forall Q: c _, (Q:Type) -> Q). 
+*)
+
+Record SClass {A:Type} (h:A) := {get : A := h}.
+Arguments get {A h} _.
+
+Class Test'
+       `(super: SClass build)
+  :=
+    { 
+      d : (get super).(c) ;
+      e : d
+    }.
+
+Record TestClone := { from : Test}.
+
+Canonical tosuper `(t:Test' super): TestClone := {| from := get super |}.
+
+Definition f (t:TestClone) (x:c (from t)) := x.
+
+Definition g1 `(t:Test' super)(x:Type) := option x.
+Definition g2 `(t:Test' super)(x:c (get super)) := option x.
+
+(* Ne marche plus *)
+
+Definition h1 `(t:Test' super)(x:Type) := option (f _ x).
+Definition h2 `(t:Test' super)(x:c (get super)) := option (f _ x).
