v4/SemanticsNE.v
@@ -1,0 +1,65 @@
+Set Implicit Arguments.
+Unset Strict Implicit.
+Set Maximal Implicit Insertion.
+Unset Printing Implicit Defensive.
+
+Require Import ssreflect Basic LAF List Coq.Program.Equality Semantics.
+
+Record ValuesSystem(MW : RealisabilityAlg) :=
+  {
+    isVal    : MW.(SNeg) -> Prop;
+    orthVal  : forall tn tp, orth (tn,tp) -> isVal tn ;
+    nonempty : forall st l (Delta:TypingDec st l) tl, exists v, SemTDec (M:=MW) Delta tl v;
+    isValtriv {w}:
+      forall rho (f:Reifiable w),
+        (forall p c, f p =cis= c -> isVal (SemN rho (rei f)))
+        -> isVal (SemN rho (rei f))
+  }.
+
+Theorem TypedIsVal (M : FullModel) (VS: ValuesSystem M):
+  forall (w:World LAF) (Gamma:TContext w) (rho:M.(SContexts) w) nt A,
+    NegTyping Gamma nt A ->  SemCont Gamma rho -> VS.(isVal) (SemN rho nt)
+.
+Proof.
+  move => w Gamma rho nt A H0 H1.
+  case: (adequacy M Gamma) => _ [_ [H _]].
+  move:(H nt A H0 rho H1).
+  move: H => _ .
+  rewrite /Pard/SemNeg/getA/getTerms.
+  case: H0 => /=; intros.
+  apply: isValtriv => p c H2.
+  move:(e p c H2).
+  clear H1 A H2 e o.
+  case => Delta H1.
+  rewrite /ortho in H.
+  case:(VS.(nonempty) Delta (SemTermList (readE rho) tl)) => v H2.
+  move: (H (tild p v)) => H3.
+  clear H.
+  have: orth (I rho f, tild p v).
+  apply:H3.
+  apply SemPosDec.
+  apply: (pv _ {{l,A0}} _ _ _ Delta) => //.
+                                     clear H3.
+  apply: orthVal.
+Qed.
+
+Print Assumptions TypedIsVal.
+
+(* Fixpoint isDecVal {st} (v:SDec st) := *)
+(*   match v with *)
+(*     | leafP xp => True *)
+(*     | leafN tm => VS.(isVal) tm *)
+(*     | dummy    => True *)
+(*     | node s1 s2 v1 v2 => isDecVal v1 /\ isDecVal v2 *)
+(*     | qnode s r v' => isDecVal v' *)
+(*   end *)
+(* . *)
+
+(* Lemma SemDecValues: forall st l (Delta:TypingDec st l) v tl, SemTDec (l := l) Delta tl v -> isDecVal v. *)
+(* Proof. *)
+(*   induction Delta; dependent induction v => tl //=. *)
+(*     by move => [H1 _]. *)
+(*     by move => [H1 H2]; split ; [apply (IHDelta1 _ tl) | apply (IHDelta2 _ tl) ]. *)
+(*     by move => [H1 H2]; apply (IHDelta _ (TermCons c Logic.I tl)). *)
+(* Qed. *)
+
